src/spec/03-theorems/corpus.lean
@@ -5,14 +5,14 @@ namespace Abstract
 open Abstract
 
 def wLag : List (Event × Nat) :=
-  [ (.external (.taskCreate { pid := "p0", ttl := 100, action := { id := oid "x", timeoutAt := 250, param := {}, tags := tgtTags } }), 100),
+  [ (.external (.taskCreate { pid := "p0", ttl := 100, action := { id := oid "x", timeoutAt := 250, param := {}, type := tgtType } }), 100),
     (.external (.taskGet { id := oid "x" }), 300),
     (.internal (.taskLeaseTimeout { id := oid "x" }), 300),
     (.internal (.taskRetryTimeout { id := oid "x" }), 300) ]
 
 def b1 : List (Event × Nat) :=
-  [ (.external (.promiseCreate { id := oid "a", timeoutAt := 1000, param := {}, tags := extTags }), 100),
-    (.external (.taskCreate { pid := "p0", ttl := 100, action := { id := oid "x", timeoutAt := 2000, param := {}, tags := tgtTags } }), 100),
+  [ (.external (.promiseCreate { id := oid "a", timeoutAt := 1000, param := {}, type := extType }), 100),
+    (.external (.taskCreate { pid := "p0", ttl := 100, action := { id := oid "x", timeoutAt := 2000, param := {}, type := tgtType } }), 100),
     (.external (.taskSuspend { id := oid "x", version := 1, actions := [{ awaited := oid "a", awaiter := oid "x" }] }), 120),
     (.external (.promiseSettle { id := oid "a", state := .resolved, value := {} }), 200),
     (.internal (.callback { awaited := oid "a", awaiter := oid "x" }), 200),
@@ -22,40 +22,40 @@ def b1 : List (Event × Nat) :=
     (.external (.taskFulfill { id := oid "x", version := 2, action := { id := oid "x", state := .resolved, value := {} } }), 230) ]
 
 def b2 : List (Event × Nat) :=
-  [ (.external (.promiseCreate { id := oid "a", timeoutAt := 1000, param := {}, tags := extTags }), 100),
-    (.external (.taskCreate { pid := "p0", ttl := 100, action := { id := oid "x", timeoutAt := 300, param := {}, tags := tgtTags } }), 100),
+  [ (.external (.promiseCreate { id := oid "a", timeoutAt := 1000, param := {}, type := extType }), 100),
+    (.external (.taskCreate { pid := "p0", ttl := 100, action := { id := oid "x", timeoutAt := 300, param := {}, type := tgtType } }), 100),
     (.external (.taskSuspend { id := oid "x", version := 1, actions := [{ awaited := oid "a", awaiter := oid "x" }] }), 120),
     (.external (.taskGet { id := oid "x" }), 500),
     (.external (.taskHalt { id := oid "x" }), 500) ]
 
 def b3 : List (Event × Nat) :=
-  [ (.external (.promiseCreate { id := oid "tm", timeoutAt := 300, param := {}, tags := timerTags }), 100),
+  [ (.external (.promiseCreate { id := oid "tm", timeoutAt := 300, param := {}, type := deadlineType }), 100),
     (.external (.promiseGet { id := oid "tm" }), 500),
     (.external (.promiseRegisterListener { awaited := oid "tm", address := "https://l" }), 500),
     (.external (.promiseSettle { id := oid "tm", state := .rejected, value := {} }), 500),
-    (.external (.promiseCreate { id := oid "tm", timeoutAt := 9999, param := {}, tags := [] }), 600) ]
+    (.external (.promiseCreate { id := oid "tm", timeoutAt := 9999, param := {}, type := .internal }), 600) ]
 
 def b4 : List (Event × Nat) :=
-  [ (.external (.taskCreate { pid := "p0", ttl := 100, action := { id := oid "y", timeoutAt := 300, param := {}, tags := tgtTags } }), 100),
+  [ (.external (.taskCreate { pid := "p0", ttl := 100, action := { id := oid "y", timeoutAt := 300, param := {}, type := tgtType } }), 100),
     (.external (.taskRelease { id := oid "y", version := 1 }), 150),
-    (.external (.taskCreate { pid := "p1", ttl := 100, action := { id := oid "y", timeoutAt := 300, param := {}, tags := tgtTags } }), 500) ]
+    (.external (.taskCreate { pid := "p1", ttl := 100, action := { id := oid "y", timeoutAt := 300, param := {}, type := tgtType } }), 500) ]
 
 def b5 : List (Event × Nat) :=
-  [ (.external (.taskCreate { pid := "p0", ttl := 1000, action := { id := oid "x", timeoutAt := 2000, param := {}, tags := tgtTags } }), 100),
-    (.external (.taskFence { id := oid "x", version := 1, action := .create { id := oid "c", timeoutAt := 3000, param := {}, tags := extTags } }), 200),
+  [ (.external (.taskCreate { pid := "p0", ttl := 1000, action := { id := oid "x", timeoutAt := 2000, param := {}, type := tgtType } }), 100),
+    (.external (.taskFence { id := oid "x", version := 1, action := .create { id := oid "c", timeoutAt := 3000, param := {}, type := extType } }), 200),
     (.external (.taskFence { id := oid "x", version := 1, action := .settle { id := oid "c", state := .resolved, value := {} } }), 300),
     (.external (.taskFence { id := oid "x", version := 1, action := .settle { id := oid "x", state := .resolved, value := {} } }), 400),
     (.external (.taskFence { id := oid "x", version := 1, action := .settle { id := oid "c", state := .resolved, value := {} } }), 2500) ]
 
 def b6 : List (Event × Nat) :=
-  [ (.external (.promiseCreate { id := oid "a", timeoutAt := 250, param := {}, tags := extTags }), 100),
+  [ (.external (.promiseCreate { id := oid "a", timeoutAt := 250, param := {}, type := extType }), 100),
     (.external (.taskGet { id := oid "a" }), 500),
     (.external (.taskHalt { id := oid "a" }), 500),
     (.external (.promiseGet { id := oid "a" }), 500) ]
 
 def kernelsResp : List Event :=
-  [ .external (.promiseCreate { id := oid "a", timeoutAt := 250, param := {}, tags := extTags }),
-    .external (.taskCreate { pid := "p0", ttl := 100, action := { id := oid "x", timeoutAt := 250, param := {}, tags := tgtTags } }),
+  [ .external (.promiseCreate { id := oid "a", timeoutAt := 250, param := {}, type := extType }),
+    .external (.taskCreate { pid := "p0", ttl := 100, action := { id := oid "x", timeoutAt := 250, param := {}, type := tgtType } }),
     .external (.taskSuspend { id := oid "x", version := 1, actions := [{ awaited := oid "a", awaiter := oid "x" }] }),
     .external (.promiseSettle { id := oid "a", state := .resolved, value := {} }),
     .external (.promiseGet { id := oid "a" }),
